ArkLib/ProofSystem/Binius/FRIBinius/CoreInteractionPhase.lean
@@ -94,7 +94,8 @@ def sumcheckFoldCtxLens : OracleContext.Lens
       let t : L⦃≤ 1⦄[X Fin ℓ'] := outerWitIn.t'
       let H : L⦃≤ 2⦄[X Fin (ℓ' - 0)] := outerWitIn.H
 
-      let P₀ : L⦃< 2^ℓ'⦄[X] := polynomialFromNovelCoeffsF₂ K β ℓ' (by omega) (fun ω => t.val.eval (bitsOfIndex ω))
+      let P₀ : L⦃< 2^ℓ'⦄[X] := polynomialFromNovelCoeffsF₂ K β ℓ' (by omega)
+        (fun ω => t.val.eval (bitsOfIndex ω))
       let f₀ : (sDomain K β (h_ℓ_add_R_rate := h_ℓ_add_R_rate))
         ⟨0, by omega⟩ → L := fun x => P₀.val.eval x.val
 
@@ -133,12 +134,14 @@ def sumcheckFoldExtractorLens : Extractor.Lens
 -- The lifted oracle verifier
 def sumcheckFoldOracleVerifier :=
   (BinaryBasefold.CoreInteraction.sumcheckFoldOracleVerifier K β (ϑ:=ϑ)
-    (h_ℓ_add_R_rate := h_ℓ_add_R_rate)).liftContext
+    (mp := RingSwitching_SumcheckMultParam κ L K (β := booleanHypercubeBasis κ L K β) ℓ ℓ' h_l)
+    (𝓑 := 𝓑) (h_ℓ_add_R_rate := h_ℓ_add_R_rate)).liftContext
       (lens := sumcheckFoldStmtLens κ L K β ℓ ℓ' 𝓡 ϑ (h_ℓ_add_R_rate := h_ℓ_add_R_rate))
 
 -- The lifted oracle reduction
 def sumcheckFoldOracleReduction :=
   (BinaryBasefold.CoreInteraction.sumcheckFoldOracleReduction K β (ϑ:=ϑ)
+    (mp := RingSwitching_SumcheckMultParam κ L K (β := booleanHypercubeBasis κ L K β) ℓ ℓ' h_l)
     (h_ℓ_add_R_rate := h_ℓ_add_R_rate) (𝓑 := 𝓑)).liftContext
       (lens := sumcheckFoldCtxLens κ L K β ℓ ℓ' 𝓡 ϑ (h_ℓ_add_R_rate := h_ℓ_add_R_rate) h_l)
 
@@ -170,22 +173,23 @@ instance sumcheckFoldCtxLens_complete :
       ℓ ℓ' h_l (𝓑 := 𝓑) (aOStmtIn := BinaryBasefoldAbstractOStmtIn κ L K β ℓ'
         𝓡 ϑ (h_ℓ_add_R_rate := h_ℓ_add_R_rate)) 0)
     (outerRelOut :=
-      BinaryBasefold.roundRelation (mp := RingSwitching_SumcheckMultParam κ L K
+      BinaryBasefold.strictRoundRelation (mp := RingSwitching_SumcheckMultParam κ L K
         (β := booleanHypercubeBasis κ L K β) ℓ ℓ' h_l) K β (ϑ:=ϑ)
         (h_ℓ_add_R_rate := h_ℓ_add_R_rate) (𝓑:=𝓑) (Fin.last ℓ')
     )
     (innerRelIn :=
-      BinaryBasefold.roundRelation (mp := RingSwitching_SumcheckMultParam κ L K
+      BinaryBasefold.strictRoundRelation (mp := RingSwitching_SumcheckMultParam κ L K
         (β := booleanHypercubeBasis κ L K β) ℓ ℓ' h_l) K β (ϑ:=ϑ)
         (h_ℓ_add_R_rate := h_ℓ_add_R_rate) (𝓑:=𝓑) 0
     )
     (innerRelOut :=
-      BinaryBasefold.roundRelation (mp := RingSwitching_SumcheckMultParam κ L K
+      BinaryBasefold.strictRoundRelation (mp := RingSwitching_SumcheckMultParam κ L K
         (β := booleanHypercubeBasis κ L K β) ℓ ℓ' h_l) K β (ϑ:=ϑ)
         (h_ℓ_add_R_rate := h_ℓ_add_R_rate) (𝓑:=𝓑) (Fin.last ℓ')
     )
     (compat :=
       let originalReduction := (CoreInteraction.sumcheckFoldOracleReduction K β (ϑ:=ϑ)
+        (mp := RingSwitching_SumcheckMultParam κ L K (β := booleanHypercubeBasis κ L K β) ℓ ℓ' h_l)
         (h_ℓ_add_R_rate := h_ℓ_add_R_rate) (𝓑 := 𝓑)).toReduction
       Reduction.compatContext (oSpec := []ₒ) (pSpec :=
         pSpecSumcheckFold K β (h_ℓ_add_R_rate := h_ℓ_add_R_rate))
@@ -214,7 +218,7 @@ theorem sumcheckFoldOracleReduction_perfectCompleteness :
       ℓ ℓ' h_l (𝓑 := 𝓑) (aOStmtIn := BinaryBasefoldAbstractOStmtIn κ L K β ℓ'
         𝓡 ϑ (h_ℓ_add_R_rate := h_ℓ_add_R_rate)) 0)
     (relOut :=
-      BinaryBasefold.roundRelation (mp := RingSwitching_SumcheckMultParam κ L K
+      BinaryBasefold.strictRoundRelation (mp := RingSwitching_SumcheckMultParam κ L K
         (β := booleanHypercubeBasis κ L K β) ℓ ℓ' h_l) K β (ϑ:=ϑ)
         (h_ℓ_add_R_rate := h_ℓ_add_R_rate) (𝓑:=𝓑) (Fin.last ℓ')
     )
@@ -244,13 +248,13 @@ theorem sumcheckFoldOracleReduction_perfectCompleteness :
     (outerRelIn := RingSwitching.sumcheckRoundRelation κ L K (booleanHypercubeBasis κ L K β)
       ℓ ℓ' h_l (𝓑 := 𝓑) (aOStmtIn := BinaryBasefoldAbstractOStmtIn κ L K β ℓ'
         𝓡 ϑ (h_ℓ_add_R_rate := h_ℓ_add_R_rate)) 0)
-    (outerRelOut := BinaryBasefold.roundRelation (mp := RingSwitching_SumcheckMultParam κ L K
+    (outerRelOut := BinaryBasefold.strictRoundRelation (mp := RingSwitching_SumcheckMultParam κ L K
       (β := booleanHypercubeBasis κ L K β) ℓ ℓ' h_l) K β (ϑ:=ϑ)
       (h_ℓ_add_R_rate := h_ℓ_add_R_rate) (𝓑:=𝓑) (Fin.last ℓ'))
-    (innerRelIn := BinaryBasefold.roundRelation (mp := RingSwitching_SumcheckMultParam κ L K
+    (innerRelIn := BinaryBasefold.strictRoundRelation (mp := RingSwitching_SumcheckMultParam κ L K
       (β := booleanHypercubeBasis κ L K β) ℓ ℓ' h_l) K β (ϑ:=ϑ)
       (h_ℓ_add_R_rate := h_ℓ_add_R_rate) (𝓑:=𝓑) 0)
-    (innerRelOut := BinaryBasefold.roundRelation (mp := RingSwitching_SumcheckMultParam κ L K
+    (innerRelOut := BinaryBasefold.strictRoundRelation (mp := RingSwitching_SumcheckMultParam κ L K
       (β := booleanHypercubeBasis κ L K β) ℓ ℓ' h_l) K β (ϑ:=ϑ)
       (h_ℓ_add_R_rate := h_ℓ_add_R_rate) (𝓑:=𝓑) (Fin.last ℓ'))
     (lens := sumcheckFoldCtxLens κ L K β ℓ ℓ' 𝓡 ϑ (h_ℓ_add_R_rate := h_ℓ_add_R_rate) h_l)
@@ -285,17 +289,17 @@ instance sumcheckFoldExtractorLens_rbr_knowledge_soundness :
       (outerRelOut :=
         BinaryBasefold.roundRelation (mp := RingSwitching_SumcheckMultParam κ L K
           (β := booleanHypercubeBasis κ L K β) ℓ ℓ' h_l) K β (ϑ:=ϑ)
-          (h_ℓ_add_R_rate := h_ℓ_add_R_rate) (𝓑:=𝓑) (Fin.last ℓ')
+          (h_ℓ_add_R_rate := h_ℓ_add_R_rate) (𝓑:=𝓑)  (Fin.last ℓ')
       )
       (innerRelIn :=
         BinaryBasefold.roundRelation (mp := RingSwitching_SumcheckMultParam κ L K
           (β := booleanHypercubeBasis κ L K β) ℓ ℓ' h_l) K β (ϑ:=ϑ)
-          (h_ℓ_add_R_rate := h_ℓ_add_R_rate) (𝓑:=𝓑) 0
+          (h_ℓ_add_R_rate := h_ℓ_add_R_rate) (𝓑:=𝓑)  0
       )
       (innerRelOut :=
         BinaryBasefold.roundRelation (mp := RingSwitching_SumcheckMultParam κ L K
           (β := booleanHypercubeBasis κ L K β) ℓ ℓ' h_l) K β (ϑ:=ϑ)
-          (h_ℓ_add_R_rate := h_ℓ_add_R_rate) (𝓑:=𝓑) (Fin.last ℓ')
+          (h_ℓ_add_R_rate := h_ℓ_add_R_rate) (𝓑:=𝓑)  (Fin.last ℓ')
       )
       (compatStmt := fun _ _ => True)
       (compatWit := fun _ _ => True)
@@ -325,9 +329,9 @@ theorem sumcheckFoldOracleVerifier_rbrKnowledgeSoundness [Fintype L] :
       (relOut :=
         BinaryBasefold.roundRelation (mp := RingSwitching_SumcheckMultParam κ L K
           (β := booleanHypercubeBasis κ L K β) ℓ ℓ' h_l) K β (ϑ:=ϑ)
-          (h_ℓ_add_R_rate := h_ℓ_add_R_rate) (𝓑:=𝓑) (Fin.last ℓ')
+          (h_ℓ_add_R_rate := h_ℓ_add_R_rate) (𝓑:=𝓑)  (Fin.last ℓ')
       )
-      (verifier := sumcheckFoldOracleVerifier κ L K β ℓ ℓ' 𝓡 ϑ
+      (verifier := sumcheckFoldOracleVerifier κ L K β ℓ ℓ' (h_l := h_l) (𝓑 := 𝓑) 𝓡 ϑ
         (h_ℓ_add_R_rate := h_ℓ_add_R_rate))
       (init := init)
       (impl := impl)
@@ -463,10 +467,11 @@ theorem finalSumcheckOracleReduction_perfectCompleteness {σ : Type}
   (impl : QueryImpl []ₒ (StateT σ ProbComp)) :
   OracleReduction.perfectCompleteness
     (pSpec := BinaryBasefold.pSpecFinalSumcheckStep (L:=L))
-    (relIn := BinaryBasefold.roundRelation (mp := RingSwitching_SumcheckMultParam κ L K
+    (relIn := BinaryBasefold.strictRoundRelation (mp := RingSwitching_SumcheckMultParam κ L K
       (β := booleanHypercubeBasis κ L K β) ℓ ℓ' h_l) K β (ϑ:=ϑ)
       (h_ℓ_add_R_rate := h_ℓ_add_R_rate) (𝓑:=𝓑) (Fin.last ℓ'))
-    (relOut := BinaryBasefold.finalSumcheckRelOut K β (ϑ:=ϑ) (h_ℓ_add_R_rate := h_ℓ_add_R_rate))
+    (relOut := BinaryBasefold.strictFinalSumcheckRelOut K β (ϑ:=ϑ)
+      (h_ℓ_add_R_rate := h_ℓ_add_R_rate))
     (oracleReduction := finalSumcheckOracleReduction κ L K β ℓ ℓ' 𝓡 ϑ
       (h_ℓ_add_R_rate := h_ℓ_add_R_rate) h_l)
     (init := init) (impl := impl) := by
@@ -526,10 +531,10 @@ def finalSumcheckKStateProp {m : Fin (1 + 1)} (tr : Transcript m (pSpecFinalSumc
       (h_ℓ_add_R_rate := h_ℓ_add_R_rate) ϑ (Fin.last ℓ') j) : Prop :=
   match m with
   | ⟨0, _⟩ => -- same as relIn
-    BinaryBasefold.masterKStateProp K β (h_ℓ_add_R_rate := h_ℓ_add_R_rate) (𝓑 := 𝓑)
+    BinaryBasefold.masterKStateProp K β (h_ℓ_add_R_rate := h_ℓ_add_R_rate)
       (mp := RingSwitching_SumcheckMultParam κ L K
         (β := booleanHypercubeBasis κ L K β) ℓ ℓ' h_l)
-      (stmtIdx := Fin.last ℓ') (oracleIdx := Fin.last ℓ') (h_le := le_refl _)
+      (stmtIdx := Fin.last ℓ') (oracleIdx := OracleFrontierIndex.mkFromStmtIdx (Fin.last ℓ'))
       (stmt := stmt) (wit := witMid) (oStmt := oStmt) (localChecks := True)
   | ⟨1, _⟩ => -- implied by relOut + local checks via extractOut proofs
     let tr_so_far := (pSpecFinalSumcheckStep (L := L)).take 1 (by omega)
@@ -552,7 +557,7 @@ def finalSumcheckKStateProp {m : Fin (1 + 1)} (tr : Transcript m (pSpecFinalSumc
     let sumcheckFinalCheck : Prop := stmt.sumcheck_target = compute_final_eq_value κ L K
       (β := booleanHypercubeBasis κ L K β) ℓ ℓ' h_l
       stmt.ctx.t_eval_point stmt.challenges stmt.ctx.r_batching * s'
-    let finalFoldingProp := finalNonDoomedFoldingProp K β (ϑ := ϑ)
+    let finalFoldingProp := finalFoldingStateProp K β (ϑ := ϑ)
       (h_ℓ_add_R_rate := h_ℓ_add_R_rate) (h_le := by
         apply Nat.le_of_dvd;
         · exact Nat.pos_of_neZero ℓ'
@@ -572,8 +577,10 @@ noncomputable def finalSumcheckKnowledgeStateFunction {σ : Type} (init : ProbCo
   where
   toFun := fun m ⟨stmt, oStmt⟩ tr witMid =>
     finalSumcheckKStateProp κ L K β ℓ ℓ' 𝓡 ϑ h_ℓ_add_R_rate h_l
-      (𝓑 := 𝓑) (tr := tr) (stmt := stmt) (witMid := witMid) (oStmt := oStmt)
-  toFun_empty := fun stmt witMid => by simp only; rfl
+      (tr := tr) (stmt := stmt) (witMid := witMid) (oStmt := oStmt)
+  toFun_empty := fun stmt witMid => by
+    -- sumcheck consistency is trivial since there is no variables left
+    sorry
   toFun_next := fun m hDir stmt tr msg witMid h => by
     -- Either bad events exist, or (oracleFoldingConsistency is true so
       -- the extractor can construct a satisfying witness)
@@ -614,8 +621,8 @@ def coreInteractionOracleVerifier :=
       (h_ℓ_add_R_rate := h_ℓ_add_R_rate) ϑ (Fin.last ℓ'))
     (pSpec₁ := BinaryBasefold.pSpecSumcheckFold K β (h_ℓ_add_R_rate := h_ℓ_add_R_rate))
     (pSpec₂ := pSpecFinalSumcheckStep (L:=L))
-    (V₁ := sumcheckFoldOracleVerifier κ L K β ℓ ℓ' 𝓡 ϑ
-        (h_ℓ_add_R_rate := h_ℓ_add_R_rate))
+    (V₁ := sumcheckFoldOracleVerifier κ (L := L) (K := K) (β := β) (ℓ := ℓ) (ℓ' := ℓ') (h_l := h_l)
+      (𝓑 := 𝓑) (𝓡 := 𝓡) (ϑ := ϑ) (h_ℓ_add_R_rate := h_ℓ_add_R_rate))
     (V₂ := finalSumcheckVerifier κ L K β ℓ ℓ' 𝓡 ϑ h_ℓ_add_R_rate h_l)
 
 /-- The final oracle reduction that composes sumcheckFold with finalSumcheckStep -/
@@ -649,10 +656,12 @@ theorem coreInteractionOracleReduction_perfectCompleteness :
       (OStmtIn := BinaryBasefold.OracleStatement K β (h_ℓ_add_R_rate := h_ℓ_add_R_rate) ϑ 0)
       (OStmtOut := BinaryBasefold.OracleStatement K β
       (h_ℓ_add_R_rate := h_ℓ_add_R_rate) ϑ (Fin.last ℓ'))
-      (relIn := RingSwitching.sumcheckRoundRelation κ L K (booleanHypercubeBasis κ L K β)
-        ℓ ℓ' h_l (𝓑 := 𝓑) (aOStmtIn := BinaryBasefoldAbstractOStmtIn κ L K β ℓ'
+      (relIn := RingSwitching.sumcheckRoundRelation κ (L := L) (K := K)
+        (β := booleanHypercubeBasis κ L K β) ℓ ℓ' h_l (𝓑 := 𝓑)
+        (aOStmtIn := BinaryBasefoldAbstractOStmtIn κ L K β ℓ'
           𝓡 ϑ (h_ℓ_add_R_rate := h_ℓ_add_R_rate)) 0)
-      (relOut := BinaryBasefold.finalSumcheckRelOut K β (ϑ:=ϑ) (h_ℓ_add_R_rate := h_ℓ_add_R_rate))
+      (relOut := BinaryBasefold.strictFinalSumcheckRelOut K β (ϑ:=ϑ)
+        (h_ℓ_add_R_rate := h_ℓ_add_R_rate))
       (oracleReduction := coreInteractionOracleReduction κ L K β ℓ ℓ' 𝓡 ϑ
         (h_ℓ_add_R_rate := h_ℓ_add_R_rate) h_l (𝓑 := 𝓑))
       (init := init)
@@ -676,8 +685,8 @@ def coreInteractionOracleRbrKnowledgeError (j : (BinaryBasefold.pSpecCoreInterac
 
 /-- Round-by-round knowledge soundness for the core interaction oracle verifier -/
 theorem coreInteractionOracleVerifier_rbrKnowledgeSoundness :
-    (coreInteractionOracleVerifier κ L K β ℓ ℓ' 𝓡 ϑ h_ℓ_add_R_rate
-      h_l).rbrKnowledgeSoundness init impl
+    (coreInteractionOracleVerifier κ (L := L) (K := K) (β := β) (ℓ := ℓ) (ℓ' := ℓ') (h_l := h_l)
+      (𝓡 := 𝓡) (ϑ := ϑ) (h_ℓ_add_R_rate := h_ℓ_add_R_rate) (𝓑 := 𝓑)).rbrKnowledgeSoundness init impl
       (OStmtIn := BinaryBasefold.OracleStatement K β (h_ℓ_add_R_rate := h_ℓ_add_R_rate) ϑ 0)
       (OStmtOut := BinaryBasefold.OracleStatement K β
       (h_ℓ_add_R_rate := h_ℓ_add_R_rate) ϑ (Fin.last ℓ'))
@@ -688,7 +697,7 @@ theorem coreInteractionOracleVerifier_rbrKnowledgeSoundness :
       (relOut := BinaryBasefold.finalSumcheckRelOut K β (ϑ:=ϑ) (h_ℓ_add_R_rate := h_ℓ_add_R_rate))
       (rbrKnowledgeError := coreInteractionOracleRbrKnowledgeError κ L K β ℓ' 𝓡 ϑ
         (h_ℓ_add_R_rate := h_ℓ_add_R_rate)) := by
-  apply OracleVerifier.append_rbrKnowledgeSoundness
+  let res := OracleVerifier.append_rbrKnowledgeSoundness
     (oSpec := []ₒ)
     (OStmt₁ := BinaryBasefold.OracleStatement K β (h_ℓ_add_R_rate := h_ℓ_add_R_rate) ϑ 0)
     (OStmt₂ := BinaryBasefold.OracleStatement K β
@@ -703,8 +712,8 @@ theorem coreInteractionOracleVerifier_rbrKnowledgeSoundness :
       (β := booleanHypercubeBasis κ L K β) ℓ ℓ' h_l) K β (ϑ:=ϑ)
       (h_ℓ_add_R_rate := h_ℓ_add_R_rate) (𝓑:=𝓑) (Fin.last ℓ'))
     (rel₃ := finalSumcheckRelOut K β (ϑ:=ϑ) (h_ℓ_add_R_rate := h_ℓ_add_R_rate))
-    (V₁ := sumcheckFoldOracleVerifier κ L K β ℓ ℓ' 𝓡 ϑ
-        (h_ℓ_add_R_rate := h_ℓ_add_R_rate))
+    (V₁ := sumcheckFoldOracleVerifier κ (L := L) (K := K) (β := β) (ℓ := ℓ) (ℓ' := ℓ') (h_l := h_l)
+      (𝓑 := 𝓑) (𝓡 := 𝓡) (ϑ := ϑ) (h_ℓ_add_R_rate := h_ℓ_add_R_rate))
     (V₂ := finalSumcheckVerifier κ L K β ℓ ℓ' 𝓡 ϑ h_ℓ_add_R_rate h_l)
     (Oₛ₃:=by exact fun i ↦ by exact OracleInterface.instDefault)
     (rbrKnowledgeError₁ := BinaryBasefold.CoreInteraction.sumcheckFoldKnowledgeError
@@ -712,6 +721,7 @@ theorem coreInteractionOracleVerifier_rbrKnowledgeSoundness :
     (rbrKnowledgeError₂ := finalSumcheckKnowledgeError (L := L))
     (h₁ := by apply sumcheckFoldOracleVerifier_rbrKnowledgeSoundness)
     (h₂ := by apply finalSumcheckOracleVerifier_rbrKnowledgeSoundness)
+  exact res
 
 end CoreInteractionPhaseReduction
 
