ArkLib/ProofSystem/Binius/BinaryBasefold/CoreInteractionPhase.lean
@@ -167,9 +167,9 @@ theorem foldRelayOracleVerifier_rbrKnowledgeSoundness
     (foldRelayOracleVerifier 𝔽q β (mp := mp) (h_ℓ_add_R_rate := h_ℓ_add_R_rate) (𝓑:=𝓑) i hNCR).rbrKnowledgeSoundness
       init impl
       (relIn := roundRelation 𝔽q β (ϑ:=ϑ) (h_ℓ_add_R_rate := h_ℓ_add_R_rate)
-        (𝓑:=𝓑) i.castSucc (includeBadEvents := true) (mp := mp))
+        (𝓑:=𝓑) i.castSucc  (mp := mp))
       (relOut := roundRelation 𝔽q β (ϑ:=ϑ) (h_ℓ_add_R_rate := h_ℓ_add_R_rate)
-        (𝓑:=𝓑) i.succ (includeBadEvents := true) (mp := mp))
+        (𝓑:=𝓑) i.succ  (mp := mp))
       (rbrKnowledgeError := fun m => foldKnowledgeError 𝔽q β (ϑ:=ϑ)
         (h_ℓ_add_R_rate := h_ℓ_add_R_rate) i ⟨m, by
         match m with
@@ -262,9 +262,9 @@ theorem foldCommitOracleVerifier_rbrKnowledgeSoundness
     (foldCommitOracleVerifier 𝔽q β (mp := mp) (h_ℓ_add_R_rate := h_ℓ_add_R_rate) (𝓑:=𝓑) i hCR).rbrKnowledgeSoundness
       init impl
       (relIn := roundRelation (mp := mp) 𝔽q β (ϑ:=ϑ)
-        (h_ℓ_add_R_rate := h_ℓ_add_R_rate) (𝓑:=𝓑) i.castSucc (includeBadEvents := true))
+        (h_ℓ_add_R_rate := h_ℓ_add_R_rate) (𝓑:=𝓑) i.castSucc )
       (relOut := roundRelation (mp := mp) 𝔽q β (ϑ:=ϑ)
-        (h_ℓ_add_R_rate := h_ℓ_add_R_rate) (𝓑:=𝓑) i.succ (includeBadEvents := true))
+        (h_ℓ_add_R_rate := h_ℓ_add_R_rate) (𝓑:=𝓑) i.succ )
       (rbrKnowledgeError := fun _ => foldKnowledgeError 𝔽q β (ϑ:=ϑ)
         (h_ℓ_add_R_rate := h_ℓ_add_R_rate) i ⟨1, by rfl⟩
       ) := by
@@ -1181,9 +1181,9 @@ theorem sumcheckFoldOracleVerifier_rbrKnowledgeSoundness :
     (sumcheckFoldOracleVerifier 𝔽q β (mp := mp) (𝓑 := 𝓑)).rbrKnowledgeSoundness init impl
       (pSpec := pSpecSumcheckFold 𝔽q β (ϑ:=ϑ) (h_ℓ_add_R_rate := h_ℓ_add_R_rate))
       (relIn := roundRelation (mp := mp) 𝔽q β (ϑ:=ϑ)
-        (h_ℓ_add_R_rate := h_ℓ_add_R_rate) (𝓑:=𝓑) 0 (includeBadEvents := true))
+        (h_ℓ_add_R_rate := h_ℓ_add_R_rate) (𝓑:=𝓑) 0 )
       (relOut := roundRelation (mp := mp) 𝔽q β (ϑ:=ϑ)
-        (h_ℓ_add_R_rate := h_ℓ_add_R_rate) (𝓑:=𝓑) (Fin.last ℓ) (includeBadEvents := true))
+        (h_ℓ_add_R_rate := h_ℓ_add_R_rate) (𝓑:=𝓑) (Fin.last ℓ) )
       (rbrKnowledgeError := sumcheckFoldKnowledgeError 𝔽q β (ϑ:=ϑ)) := by
   unfold sumcheckFoldOracleVerifier pSpecSumcheckFold
   sorry
@@ -1270,15 +1270,15 @@ theorem coreInteractionOracleVerifier_rbrKnowledgeSoundness :
     (coreInteractionOracleVerifier 𝔽q β (𝓑 := 𝓑)).rbrKnowledgeSoundness init impl
       (pSpec := pSpecCoreInteraction 𝔽q β (h_ℓ_add_R_rate := h_ℓ_add_R_rate))
       (relIn := roundRelation (mp := BBF_SumcheckMultiplierParam) 𝔽q β (ϑ:=ϑ)
-        (h_ℓ_add_R_rate := h_ℓ_add_R_rate) (𝓑:=𝓑) 0 (includeBadEvents := true))
-      (relOut := finalSumcheckRelOut 𝔽q β (ϑ:=ϑ) (h_ℓ_add_R_rate := h_ℓ_add_R_rate) (includeBadEvents := true))
+        (h_ℓ_add_R_rate := h_ℓ_add_R_rate) (𝓑:=𝓑) 0 )
+      (relOut := finalSumcheckRelOut 𝔽q β (ϑ:=ϑ) (h_ℓ_add_R_rate := h_ℓ_add_R_rate) )
       (rbrKnowledgeError := coreInteractionOracleRbrKnowledgeError 𝔽q β (ϑ:=ϑ)) := by
   unfold coreInteractionOracleVerifier pSpecCoreInteraction
   apply OracleVerifier.append_rbrKnowledgeSoundness
     (init:=init) (impl:=impl)
-    (rel₁ := roundRelation 𝔽q β (ϑ:=ϑ) (h_ℓ_add_R_rate := h_ℓ_add_R_rate) (𝓑:=𝓑) 0 (includeBadEvents := true))
-    (rel₂ := roundRelation 𝔽q β (ϑ:=ϑ) (h_ℓ_add_R_rate := h_ℓ_add_R_rate) (𝓑:=𝓑) (Fin.last ℓ) (includeBadEvents := true))
-    (rel₃ := finalSumcheckRelOut 𝔽q β (ϑ:=ϑ) (h_ℓ_add_R_rate := h_ℓ_add_R_rate) (includeBadEvents := true))
+    (rel₁ := roundRelation 𝔽q β (ϑ:=ϑ) (h_ℓ_add_R_rate := h_ℓ_add_R_rate) (𝓑:=𝓑) 0 )
+    (rel₂ := roundRelation 𝔽q β (ϑ:=ϑ) (h_ℓ_add_R_rate := h_ℓ_add_R_rate) (𝓑:=𝓑) (Fin.last ℓ) )
+    (rel₃ := finalSumcheckRelOut 𝔽q β (ϑ:=ϑ) (h_ℓ_add_R_rate := h_ℓ_add_R_rate) )
     (V₁ := sumcheckFoldOracleVerifier 𝔽q β
       (h_ℓ_add_R_rate := h_ℓ_add_R_rate) (ϑ:=ϑ))
     (V₂ := finalSumcheckVerifier 𝔽q β
